finish implementing interpreter

coq/theories/Interp.v
@@ -1,6 +1,8 @@
+Require Import Coq.Program.Program.
 Require Import Coq.Classes.EquivDec.
 Require Import Coq.Lists.List.
 Import List.ListNotations.
+Require Import Coq.NArith.NArith.
 Require Import MiniP4.Syntax.
 
 Axiom hash: list bool -> list bool.
@@ -21,21 +23,56 @@ Definition both_some {A B: Type} (a: option A) (b: option B) : option (A * B) :=
   | _, _ => None
   end.
 
-Definition bitstring_eq_dec (b1 b2: bitstring) : {b1 = b2} + {b1 <> b2}.
-Admitted.
-Definition val_eq_dec (v1 v2: val) : {v1 = v2} + {v1 <> v2}.
-Admitted.
+Instance bitstring_eq_dec: EqDec bitstring eq := ltac:(typeclasses eauto).
+Program Fixpoint val_eqdec (x y: val) : {x = y} + {x <> y} :=
+  match x, y with
+  | VBits xs, VBits ys => if xs == ys then in_left else in_right
+  | VBool x, VBool y => if x == y then in_left else in_right
+  | VTuple xs, VTuple ys => if list_eq_dec val_eqdec xs ys then in_left else in_right
+  | _, _ => in_right
+  end.
+Next Obligation.
+  congruence.
+Qed.
+Next Obligation.
+  congruence.
+Qed.
+Next Obligation.
+  intro; subst.
+  destruct y.
+  - eapply H1; auto.
+  - eapply H; auto.
+  - eapply H0; auto.
+Qed.
+Solve All Obligations with (cbn; intros; intuition congruence).
+
+Instance val_eq_dec: EqDec val eq := val_eqdec.
 
 Definition interp_binop (o: binop) '((v1, v2): val * val) : val :=
   match o with
-  | Eq => if val_eq_dec v1 v2 then VBits [true] else VBits [false]
-  | Neq => if val_eq_dec v1 v2 then VBits [false] else VBits [true]
+  | Eq => if v1 == v2 then VBits [true] else VBits [false]
+  | Neq => if v1 == v2 then VBits [false] else VBits [true]
   end.
 
-Definition to_num (l: list bool) : nat.
-Admitted.
-Definition to_list (n: nat) : list bool.
-Admitted.
+Fixpoint to_num (l: list bool) : N :=
+  match l with
+  | [] => 0
+  | true :: l => 1 + 2 * to_num l
+  | false :: l => 2 * to_num l
+  end.
+
+Fixpoint to_list_positive (n: positive) : list bool :=
+  match n with
+  | xH => [true]
+  | xO n => false :: to_list_positive n
+  | xI n => true :: to_list_positive n
+  end.
+
+Definition to_list (n: N) : list bool :=
+  match n with 
+  | N0 => [false]
+  | Npos n => to_list_positive n
+  end.
 
 Program Definition interp_uop (o: uop) (v: val) : option val :=
   match o with
@@ -49,29 +86,29 @@ Program Definition interp_uop (o: uop) (v: val) : option val :=
     | VTuple vs =>
       Some (VBits (to_list (List.fold_right (fun v acc =>
                          match v with
-                         | VBits l => to_num l + acc
+                         | VBits l => (to_num l + acc)%N
                          | _ => acc
                          end)
-                      0 vs)))
+                      0%N vs)))
     | _ => None
     end
   end.
 
-Fixpoint interp_expr (s: state) (e: exp) : option val :=
+Fixpoint interp_exp (s: state) (e: exp) : option val :=
   match e with
   | Var x => Env.find x s.(store)
   | Bits bs => Some (VBits bs)
   | Tuple exps =>
-    option_map VTuple (all_some (List.map (interp_expr s) exps))
+    option_map VTuple (all_some (List.map (interp_exp s) exps))
   | Proj e n =>
-    match interp_expr s e with
+    match interp_exp s e with
     | Some (VTuple vs) => nth_error vs n
     | _ => None
     end
   | BinOp o e1 e2 =>
-    option_map (interp_binop o) (both_some (interp_expr s e1) (interp_expr s e2))
+    option_map (interp_binop o) (both_some (interp_exp s e1) (interp_exp s e2))
   | UOp o e =>
-    match interp_expr s e with
+    match interp_exp s e with
     | Some v => interp_uop o v
     | None => None
     end
@@ -79,21 +116,112 @@ Fixpoint interp_expr (s: state) (e: exp) : option val :=
 
 Definition set_store (s: state) (e: Env.t name val) : state :=
   {| store := e;
+     type_env := s.(type_env);
      pkt := s.(pkt);
      acts := s.(acts);
      tables := s.(tables) |}.
 
-Definition interp_table (s: state) (tbl: table) (rules: list rule) : option state.
-Admitted.
+Definition set_type_env (s: state) (e: Env.t name typ) : state :=
+  {| store := s.(store);
+     type_env := e;
+     pkt := s.(pkt);
+     acts := s.(acts);
+     tables := s.(tables) |}.
 
-Program Fixpoint interp_cmd (fuel: nat) (s: state) (c: cmd) : option state :=
+Definition set_pkt (s: state) (pk: list bool) : state :=
+  {| store := s.(store);
+     type_env := s.(type_env);
+     pkt := pk;
+     acts := s.(acts);
+     tables := s.(tables) |}.
+
+Definition set_acts (s: state) (e: Env.t name action) : state :=
+  {| store := s.(store);
+     type_env := s.(type_env);
+     pkt := s.(pkt);
+     acts := e;
+     tables := s.(tables) |}.
+
+Definition set_tables (s: state) (e: Env.t name (table * list rule)) : state :=
+  {| store := s.(store);
+     type_env := s.(type_env);
+     pkt := s.(pkt);
+     acts := s.(acts);
+     tables := e |}.
+
+Definition splitn {A} (n: nat) (l: list A) : list A * list A :=
+  (firstn n l, skipn n l).
+
+Fixpoint extr (pk: list bool) (t: typ) : option (val * list bool) :=
+  match t with
+  | Bit n => 
+    let '(h, pk) := splitn n pk in
+    Some (VBits h, pk)
+  | Bool =>
+    let '(h, pk) := splitn 1 pk in
+    match h with
+    | [b] => Some (VBool b, pk)
+    | _ => None
+    end
+  | Prod ts =>
+    match List.fold_left (fun acc t =>
+                            match acc with
+                            | Some (vs, pk) =>
+                              match extr pk t with
+                              | Some (v, pk) =>
+                                Some (vs ++ [v], pk)
+                              | None => None
+                              end
+                            | None => None
+                            end) ts (Some ([], pk))
+    with
+    | Some (vs, pk) =>
+      Some (VTuple vs, pk)
+    | None =>
+      None
+    end
+  end.
+
+Definition interp_extr (s: state) (x: name) (t: typ) : option state :=
+  match extr s.(pkt) t with
+  | Some (v, pk) =>
+    Some {| store := Env.bind x v s.(store);
+            type_env := s.(type_env);
+            pkt := pk;
+            acts := s.(acts);
+            tables := s.(tables) |}
+  | None => None
+  end.
+
+Fixpoint emit (v: val) : list bool :=
+  match v with
+  | VBits bs => bs
+  | VBool b => [b]
+  | VTuple vs => List.fold_left (fun bs v => bs ++ emit v) vs []
+  end.
+
+Definition interp_emit (s: state) (v: val) : option state :=
+  let bs := emit v in
+  Some (set_pkt s bs).
+
+Fixpoint find_rule (s: state) (k: val) (rules: list rule) : option name :=
+  match rules with
+  | r :: rules =>
+    match interp_exp s r.(rule_match) with
+    | Some v => if k == v then Some r.(rule_action) else find_rule s k rules
+    | None => None
+    end
+  | [] => None
+  end.
+
+Fixpoint interp_cmd (fuel: nat) (s: state) (c: cmd) : option state :=
   match fuel with
   | 0 => None
   | S fuel =>
     match c with
     | Assign x e =>
       option_map (fun v => set_store s (Env.bind x v s.(store)))
-                 (interp_expr s e)
+                 (interp_exp s e)
     | Block cs => List.fold_right
                    (fun c s => match s with
                             | Some s => interp_cmd fuel s c
@@ -102,7 +230,7 @@ Program Fixpoint interp_cmd (fuel: nat) (s: state) (c: cmd) : option state :=
                    (Some s)
                    cs
     | If e c1 c2 =>
-      match interp_expr s e with
+      match interp_exp s e with
       | Some (VBits [true]) =>
         interp_cmd fuel s c1
       | Some _ =>
@@ -110,17 +238,77 @@ Program Fixpoint interp_cmd (fuel: nat) (s: state) (c: cmd) : option state :=
       | None =>
         None
       end
-    | Extr x => _
-    | Emit x => _
+    | Extr x => 
+      match Env.find x s.(type_env) with
+      | Some t => interp_extr s x t
+      | None => None
+      end
+    | Emit x =>
+      match Env.find x s.(store) with
+      | Some v => interp_emit s v
+      | None => None
+      end
     | Apply t =>
       match Env.find t s.(tables) with
-      | Some (tbl, rules) => interp_table s tbl rules
+      | Some (tbl, rules) => interp_table fuel s tbl rules
       | None => None
       end
     | Call a =>
-      match Env.find a s.(acts) with
-      | Some act => interp_cmd fuel s act.(body)
-      | None => None
-      end
+      interp_call fuel s a
     end
+  end
+with interp_call (fuel: nat) (s: state) (a: name) : option state :=
+       match fuel with
+       | 0 => None
+       | S fuel =>
+         match Env.find a s.(acts) with
+         | Some act => interp_cmd fuel s act.(body)
+         | None => None
+         end
+       end
+with interp_table (fuel: nat) (s: state) (tbl: table) (rules: list rule) : option state :=
+       match fuel with
+       | 0 => None
+       | S fuel =>
+         match interp_exp s tbl.(table_key) with
+         | Some key =>
+           match find_rule s key rules with
+           | Some act => interp_call fuel s act
+           | None => None
+           end
+         | None => None
+         end
+       end.
+
+Program Fixpoint interp_defn (fuel: nat) (s: state) (d: defn) : option state :=
+  match d with
+  | VarDecl t x e =>
+    option_map (fun v =>
+                  set_type_env
+                    (set_store s (Env.bind x v s.(store)))
+                    (Env.bind x t s.(type_env)))
+               (interp_exp s e)
+  | Action a c =>
+    Some (set_acts s (Env.bind a {| body := c |} s.(acts)))
+  | Table t keys actions =>
+    Some (set_tables s (Env.bind t ({| table_key:=keys; table_acts := actions |}, []) s.(tables)))
+  end.
+
+Fixpoint interp_defns (fuel: nat) (s: state) (defs: list defn) : option state :=
+  match defs with
+  | [] => Some s
+  | d :: defs =>
+    match interp_defn fuel s d with
+    | Some s => interp_defns fuel s defs
+    | None => None
+    end
+  end.
+
+Definition interp_prog (fuel: nat) (s: state) (p: prog) : option state :=
+  let '(defs, c) := p in
+  match interp_defns fuel s defs with
+  | Some s =>
+    interp_cmd fuel s c
+  | None =>
+    None
   end.
